src/go_lang/struct.v
@@ -51,6 +51,12 @@ Definition buildStruct (d:descriptor) (fvs: list (string*expr)) : expr :=
   | None => LitV LitUnit
   end.
 
+Definition allocStruct (d:descriptor) (fvs: list (string*expr)) : expr :=
+  match build_struct_val fvs (rev d.(fields)) with
+  | Some v => AllocStruct v
+  | None => LitV LitUnit
+  end.
+
 Fixpoint struct_ty_prod (rev_fields: list (string*ty)) : ty :=
   match rev_fields with
   | nil => unitT
@@ -61,21 +67,30 @@ Fixpoint struct_ty_prod (rev_fields: list (string*ty)) : ty :=
 Definition structTy (d:descriptor) : ty :=
   struct_ty_prod (rev (fields d)).
 
-Fixpoint ty_size (t:ty) : nat :=
+Fixpoint fieldTypes (fields: list (string*ty)) : list ty :=
+  match fields with
+  | [] => []
+  | (_,t)::fs => flatten_ty t ++ fieldTypes fs
+  end.
+
+Definition structRefTy (d:descriptor) : ty :=
+  structRefT (fieldTypes d.(fields)).
+
+Fixpoint ty_size (t:ty) : Z :=
   match t with
   | prodT t1 t2 => ty_size t1 + ty_size t2
   (* this gives unit values space, which seems fine *)
   | _ => 1
   end.
 
-Fixpoint load_ty (t:ty) (e:expr) : expr :=
+Fixpoint load_ty (t:ty) (e:expr) (off:Z) : expr :=
   match t with
-  | prodT t1 t2 => (load_ty t1 e, load_ty t2 (e +ₗ #(ty_size t1)))
-  | _ => !e
+  | prodT t1 t2 => (load_ty t1 e off, load_ty t2 e (off + ty_size t1))
+  | _ => !(e +ₗ #off)
   end.
 
 Definition loadStruct (d:descriptor) : val :=
-  λ: "p", load_ty (structTy d) (Var "p").
+  λ: "p", load_ty (structTy d) (Var "p") 0.
 
 Fixpoint field_offset (fields: list (string*ty)) f0 : (Z * ty) :=
   match fields with
@@ -87,7 +102,170 @@ Fixpoint field_offset (fields: list (string*ty)) f0 : (Z * ty) :=
 
 Definition loadField (d:descriptor) (f:string) : val :=
   let (off, t) := field_offset d.(fields) f in
-  λ: "p", load_ty t (Var "p" +ₗ #off).
+  λ: "p", load_ty t (Var "p") off.
+
+Fixpoint fieldTy (fs:list (string*ty)) (f0: string) : option ty :=
+  match fs with
+  | [] => None
+  | (f,t)::fs => if String.eqb f f0 then Some t else fieldTy fs f0
+  end.
+
+Context {ext_ty: ext_types ext}.
+Set Default Proof Using "ext ext_ty".
+
+Hint Resolve struct_offset_op_hasTy_eq : types.
+
+Theorem load_structRef_off : forall Γ e ts n t,
+  ts !! Z.to_nat n = Some t ->
+  (Γ ⊢ e : structRefT ts)%T ->
+  (Γ ⊢ ! (e +ₗ #n) : t)%T.
+Proof.
+  intros.
+  destruct (elem_of_list_split_length ts (Z.to_nat n) t)
+    as [l1 [l2 (?&?)]]; auto; subst.
+  eapply load_struct_hasTy.
+  eapply struct_offset_op_hasTy_eq; eauto.
+  rewrite drop_app_alt; auto.
+Qed.
+
+Hint Resolve load_structRef_off : types.
+
+Theorem take_1_drop_is_lookup n : forall A (l: list A) x,
+  take 1 (drop n l) = [x] ->
+  l !! n = Some x.
+Proof.
+  induction n; destruct l; simpl in *; auto; intros; try congruence.
+Qed.
+
+Hint Resolve take_1_drop_is_lookup : types.
+
+Lemma take_app_take1:
+  ∀ l1 l2 ts' : list ty,
+  take (strings.length l1 + strings.length l2) ts' = l1 ++ l2 ->
+  take (strings.length l1) ts' = l1.
+Proof.
+  intros l1 l2 ts' H.
+  replace (take (strings.length l1) ts') with (take (strings.length l1) (take (strings.length l1 + strings.length l2) ts')).
+  - rewrite H.
+    rewrite take_app; auto.
+  - rewrite take_take.
+    rewrite Min.min_l; try lia; auto.
+Qed.
+
+Theorem ty_size_flatten t : ty_size t = length (flatten_ty t).
+Proof.
+  induction t; simpl; auto.
+  rewrite app_length; auto.
+  lia.
+Qed.
+
+Lemma take_app_drop1:
+  ∀ (ts l1 l2 : list ty) (n' : nat),
+  take (strings.length l1 + strings.length l2) (drop n' ts) = l1 ++ l2
+  → take (strings.length l2) (drop (n' + strings.length l1) ts) = l2.
+Proof.
+  intros ts l1 l2 n' H.
+  rewrite <- drop_drop.
+  rewrite take_drop_commute.
+  rewrite H.
+  rewrite drop_app; auto.
+Qed.
+
+Theorem ty_size_gt_0 : forall t, (0 <= ty_size t)%Z.
+Proof.
+  induction t; simpl; lia.
+Qed.
+
+Theorem load_ty_t : forall Γ t ts n,
+  (0 <= n)%Z ->
+  firstn (length (flatten_ty t)) (drop (Z.to_nat n) ts) = flatten_ty t ->
+  (Γ ⊢ (λ: "p", load_ty t (Var "p") n)%V : (structRefT ts -> t))%T.
+Proof.
+  intros.
+  apply empty_context_to_any.
+  constructor.
+  constructor.
+  rewrite insert_anon.
+  generalize dependent n.
+  generalize dependent ts.
+  induction t; simpl; intros;
+    eauto with types.
+  rewrite app_length in H0.
+  constructor.
+  - apply IHt1; auto.
+    eapply take_app_take1; eauto.
+  - apply IHt2; auto.
+    pose proof (ty_size_gt_0 t1); lia.
+    rewrite ty_size_flatten.
+    generalize dependent (flatten_ty t1); intros l1 **.
+    generalize dependent (flatten_ty t2); intros l2 **.
+    replace (Z.to_nat (n + length l1)) with (Z.to_nat n + length l1)%nat; [ | lia ].
+    eapply take_app_drop1; eauto.
+Qed.
+
+Theorem field_offset1_gt_0 : forall fs f t,
+  fieldTy fs f = Some t ->
+  (0 <= (field_offset fs f).1)%Z.
+Proof.
+  induction fs; simpl; intros; eauto.
+  - congruence.
+  - destruct a as [f0 t']; simpl.
+    destruct (f0 =? f)%string; simpl in *; try lia.
+    + destruct_with_eqn (field_offset fs f).
+      eapply IHfs in H.
+      rewrite Heqp in H; simpl in *.
+      pose proof (ty_size_gt_0 t').
+      lia.
+Qed.
+
+Theorem field_offset_to_fieldTy : forall fs f z t0 t,
+  fieldTy fs f = Some t0 ->
+  field_offset fs f = (z, t) ->
+  t = t0 /\
+  exists ts1 ts2, fieldTypes fs = ts1 ++ flatten_ty t ++ ts2 /\
+             length ts1 = Z.to_nat z.
+Proof.
+  induction fs; simpl; intros.
+  - congruence.
+  - destruct a as [f0 t']; simpl in *.
+    destruct (f0 =? f)%string.
+    + inversion H0; subst; clear H0.
+      inversion H; subst; clear H.
+      intuition.
+      eexists nil, _; simpl; eauto.
+    + destruct_with_eqn (field_offset fs f).
+      inversion H0; subst; clear H0.
+      pose proof (IHfs _ _ _ _ H Heqp); intuition subst.
+      destruct H2 as (ts1&ts2&?&?).
+      rewrite H0.
+      eexists (flatten_ty t' ++ ts1), _; intuition eauto.
+      rewrite <- app_assoc; auto.
+      rewrite app_length.
+      rewrite ty_size_flatten.
+      rewrite H1.
+      pose proof (field_offset1_gt_0 fs f t0); intuition.
+      rewrite Heqp in H3; simpl in *.
+      lia.
+Qed.
+
+Theorem loadField_t : forall d f t,
+  fieldTy d.(fields) f = Some t ->
+  forall Γ, (Γ ⊢ loadField d f : (structRefTy d -> t))%T.
+Proof.
+  destruct d as [fs].
+  unfold structRefTy, loadField; simpl.
+  intros.
+  destruct_with_eqn (field_offset fs f).
+  pose proof (field_offset_to_fieldTy _ _ _ _ _ H Heqp);
+    intuition subst.
+  destruct H2 as (t1&t2&?&?).
+  rewrite H0.
+  eapply load_ty_t.
+  pose proof (field_offset1_gt_0 fs f t); intuition.
+  { rewrite Heqp in H3; simpl in *; lia. }
+  rewrite drop_app_alt; [ | lia ].
+  rewrite take_app; auto.
+Qed.
 
 End go_lang.
 
@@ -109,13 +287,15 @@ Declare Reduction buildStruct :=
        String.eqb Ascii.eqb eqb].
 
 Module struct.
-  Notation new := mkStruct.
+  Notation decl := mkStruct.
   Notation mk := buildStruct.
+  Notation new := allocStruct.
   Notation get := getField.
   (* TODO: load/loadF could probably use better names *)
   Notation load := loadStruct.
   Notation loadF := loadField.
   Notation t := structTy.
+  Notation ptrT := structRefTy.
 End struct.
 
 Notation "'structF!' desc fname" := (ltac:(make_structF desc fname))
